update

theory/Dynamic_Communication_Analysis.thy
@@ -2,45 +2,59 @@ theory Dynamic_Communication_Analysis
   imports Main Syntax Dynamic_Semantics
 begin
 
-definition is_send_path :: "trace_pool \<Rightarrow> chan \<Rightarrow> control_path \<Rightarrow> bool" where
-  "is_send_path \<E> c \<pi>\<^sub>y \<equiv> (\<exists> x\<^sub>y x\<^sub>e e\<^sub>n \<kappa> \<rho> x\<^sub>s\<^sub>c x\<^sub>m \<rho>\<^sub>e.
-    \<E> \<pi>\<^sub>y = Some (\<langle>LET x\<^sub>y = SYNC x\<^sub>e in e\<^sub>n; \<rho>; \<kappa>\<rangle>) \<and>
-    \<rho> x\<^sub>e = Some (VClosure (Send_Evt x\<^sub>s\<^sub>c x\<^sub>m) \<rho>\<^sub>e) \<and> 
-    \<rho>\<^sub>e x\<^sub>s\<^sub>c = Some (VChan c)
-  )"
+inductive is_send_path :: "trace_pool \<Rightarrow> chan \<Rightarrow> control_path \<Rightarrow> bool" where
+  "
+    \<E> \<pi>\<^sub>y = Some (\<langle>LET x\<^sub>y = SYNC x\<^sub>e in e\<^sub>n; \<rho>; \<kappa>\<rangle>) \<Longrightarrow>
+    \<rho> x\<^sub>e = Some (VClosure (Send_Evt x\<^sub>s\<^sub>c x\<^sub>m) \<rho>\<^sub>e) \<Longrightarrow>
+    \<rho>\<^sub>e x\<^sub>s\<^sub>c = Some (VChan c) \<Longrightarrow>
+    is_send_path \<E> c \<pi>\<^sub>y
+  "
 
-definition is_recv_path :: "trace_pool \<Rightarrow> chan \<Rightarrow> control_path \<Rightarrow> bool" where
-  "is_recv_path \<E> c \<pi>\<^sub>y \<equiv> (\<exists> x\<^sub>y x\<^sub>e e\<^sub>n \<kappa> \<rho> x\<^sub>r\<^sub>c \<rho>\<^sub>e.
-    \<E> \<pi>\<^sub>y = Some (\<langle>LET x\<^sub>y = SYNC x\<^sub>e in e\<^sub>n; \<rho>; \<kappa>\<rangle>) \<and> 
-    \<rho> x\<^sub>e = Some (VClosure (Recv_Evt x\<^sub>r\<^sub>c) \<rho>\<^sub>e) \<and> 
-    \<rho>\<^sub>e x\<^sub>r\<^sub>c = Some (VChan c)
-  )"
+inductive is_recv_path :: "trace_pool \<Rightarrow> chan \<Rightarrow> control_path \<Rightarrow> bool" where
+  "
+    \<E> \<pi>\<^sub>y = Some (\<langle>LET x\<^sub>y = SYNC x\<^sub>e in e\<^sub>n; \<rho>; \<kappa>\<rangle>) \<Longrightarrow>
+    \<rho> x\<^sub>e = Some (VClosure (Recv_Evt x\<^sub>r\<^sub>c) \<rho>\<^sub>e) \<Longrightarrow>
+    \<rho>\<^sub>e x\<^sub>r\<^sub>c = Some (VChan c) \<Longrightarrow>
+    is_recv_path \<E> c \<pi>\<^sub>y
+  "
 
 
-definition all  :: "(control_path \<Rightarrow> bool) \<Rightarrow> (control_path \<Rightarrow> control_path \<Rightarrow> bool) \<Rightarrow> bool" where
-  "all P R \<equiv> (\<forall> \<pi>\<^sub>1 \<pi>\<^sub>2 .
-    P \<pi>\<^sub>1 \<longrightarrow>
-    P \<pi>\<^sub>2 \<longrightarrow>
-    R \<pi>\<^sub>1 \<pi>\<^sub>2
-  )"
+inductive all  :: "(control_path \<Rightarrow> bool) \<Rightarrow> (control_path \<Rightarrow> control_path \<Rightarrow> bool) \<Rightarrow> bool" where
+  "
+    (\<forall> \<pi>\<^sub>1 \<pi>\<^sub>2 .
+      P \<pi>\<^sub>1 \<longrightarrow>
+      P \<pi>\<^sub>2 \<longrightarrow>
+      R \<pi>\<^sub>1 \<pi>\<^sub>2
+    ) \<Longrightarrow>
+    all P R
+  "
 
 fun ordered where
   "ordered \<pi>\<^sub>1 \<pi>\<^sub>2 = (prefix \<pi>\<^sub>1 \<pi>\<^sub>2 \<or> prefix \<pi>\<^sub>2 \<pi>\<^sub>1)"
 
-definition one_shot :: "trace_pool \<Rightarrow> chan \<Rightarrow> bool" where
-  "one_shot \<E> c \<equiv> all (is_send_path \<E> c) op="
+inductive one_shot :: "trace_pool \<Rightarrow> chan \<Rightarrow> bool" where
+  "all (is_send_path \<E> c) op= \<Longrightarrow> one_shot \<E> c"
 
 
-definition one_to_one :: "trace_pool \<Rightarrow> chan \<Rightarrow> bool" where
-  "one_to_one \<E> c \<equiv> all (is_send_path \<E> c) ordered \<and> all (is_recv_path \<E> c) ordered"
+inductive one_to_one :: "trace_pool \<Rightarrow> chan \<Rightarrow> bool" where
+  "
+    all (is_send_path \<E> c) ordered \<and> all (is_recv_path \<E> c) ordered \<Longrightarrow> 
+    one_to_one \<E> c
+  "
   
 
-definition fan_out :: "trace_pool \<Rightarrow> chan \<Rightarrow> bool" where
-  "fan_out \<E> c \<equiv> all (is_send_path \<E> c) ordered"
-  
+inductive fan_out :: "trace_pool \<Rightarrow> chan \<Rightarrow> bool" where
+  "
+    all (is_send_path \<E> c) ordered \<Longrightarrow>
+    fan_out \<E> c
+  "
 
-definition fan_in :: "trace_pool \<Rightarrow> chan \<Rightarrow> bool" where
-  "fan_in \<E> c \<equiv> all (is_recv_path \<E> c) ordered"
+  
+inductive fan_in :: "trace_pool \<Rightarrow> chan \<Rightarrow> bool" where
+  "
+    all (is_recv_path \<E> c) ordered \<Longrightarrow> 
+    fan_in \<E> c
+  "
 
 
 end
