theory/Static_Framework.thy
@@ -148,203 +148,29 @@ inductive static_flow_set :: "abstract_value_env \<Rightarrow> flow_set \<Righta
     static_flow_set \<V> \<F> (LET x = APP f x\<^sub>a in e)
   "
 
-inductive is_subexp :: "exp \<Rightarrow> exp \<Rightarrow> bool"  where
+inductive is_super_exp :: "exp \<Rightarrow> exp \<Rightarrow> bool"  where
   Refl : "
-    is_subexp e e
+    is_super_exp e e
   " | 
   Let: "
-    is_subexp e\<^sub>n e \<Longrightarrow>
-    is_subexp (LET x = b in e\<^sub>n) e
+    is_super_exp e\<^sub>n e \<Longrightarrow>
+    is_super_exp (LET x = b in e\<^sub>n) e
   " | 
   Let_Spawn_Child: "
-    is_subexp e\<^sub>c e \<Longrightarrow>
-    is_subexp (LET x = SPAWN e\<^sub>c in e\<^sub>n) e
+    is_super_exp e\<^sub>c e \<Longrightarrow>
+    is_super_exp (LET x = SPAWN e\<^sub>c in e\<^sub>n) e
   " |
   Let_Case_Left: "
-    is_subexp e\<^sub>l e \<Longrightarrow>
-    is_subexp (LET x = CASE x\<^sub>s LEFT x\<^sub>l |> e\<^sub>l RIGHT x\<^sub>r |> e\<^sub>r in e\<^sub>n) e
+    is_super_exp e\<^sub>l e \<Longrightarrow>
+    is_super_exp (LET x = CASE x\<^sub>s LEFT x\<^sub>l |> e\<^sub>l RIGHT x\<^sub>r |> e\<^sub>r in e\<^sub>n) e
   " |
   Let_Case_Right: "
-    is_subexp e\<^sub>r e \<Longrightarrow>
-    is_subexp (LET x = CASE x\<^sub>s LEFT x\<^sub>l |> e\<^sub>l RIGHT x\<^sub>r |> e\<^sub>r in e\<^sub>n) e
+    is_super_exp e\<^sub>r e \<Longrightarrow>
+    is_super_exp (LET x = CASE x\<^sub>s LEFT x\<^sub>l |> e\<^sub>l RIGHT x\<^sub>r |> e\<^sub>r in e\<^sub>n) e
   " |
   Let_Abs_Body: "
-    is_subexp e\<^sub>b e \<Longrightarrow>
-    is_subexp (LET x = FN f x\<^sub>p . e\<^sub>b in e\<^sub>n) e
+    is_super_exp e\<^sub>b e \<Longrightarrow>
+    is_super_exp (LET x = FN f x\<^sub>p . e\<^sub>b in e\<^sub>n) e
   "
-
-
-(* TO DO: ensure that the abstract value env doesn't need hold values of new spawn variables*)
-(* find channel creation subexpressions*)
-(* transforming LET x = SYNC xSE in e into LET x = SPAWN eCh in e, should work*)
-(* How to determine eCh? Find the SYNC RECV EVT sub expression, where channel values send site's values*)
-
-(*
-
-Xiao says "
-The next definition
-and lemma show that for each dynamic send/receive site of
-any channel instance, there is a corresponding approximate path in
-the extended CFG, which starts from the channel’s creation site
-(TLL modification: or from ad-hoc spawn expression to tie in sync recv_evts into corresponding chan expression with sync send_evt)
-"
-
-dynamic flow of channel instance:
-let \<pi> \<in> Sendst(k)
-PathHtk(\<pi>) = \<langle>\<pi>1, \<pi>2\<rangle>. This means that
-\<pi>1(1)
-1 is the creation site of k, k flows through \<pi>1 and then is sent as
-a message from \<pi>1(−1) to \<pi>2(1) on some channel instance, and some
-value is sent on k at \<pi>2(−1) is a send on k.
-
-for every dynamic path to a send or recv site in an expression,
-there is a corresponding modified path in a corresponding modified expression.
-
-
-Q: Need to modify dynamic semantics with history of communication?
-A: Seems like the only reason is because modified paths use 
-the sender's front with receiver's back for passed channels.  
-We can simply use the back, the path of which is already recorded in the trace_pool.
-
-(\<pi>Send, Ch \<pi>C xC, \<pi>Recv)
-
-Xiao says:
-
-"
-Lemma 6 For any trace t 2 Trace(p), channel instance k in t, and any control path \<pi>1, \<pi>2 2
-Sendst(k) [ Recvst(k), if \<pi>1 6= \<pi>2 then PathHtk(\<pi>1) 6= PathHtk(\<pi>2).
-
-Proof: This is obvious from dynamic semantics on Section 3.1.
-"
-
-Need to consider only subprograms where channel is live.o
-
-Check how Xiao proves that graph of subprogram actually represents the whole program.
-
-strategy 1:
-Find all the fragments that start with (LET x = CHAN \<lparr>\<rparr> in e).
-Find all the fragments that start with (LET x = RECV eRE in e).
-join fragments with initial (LET * = SPAWN (LET x = RECV eRE in) in (LET x = CHAN \<lparr>\<rparr> in e))
-
-incomplete strategy 2:
-Transform 
-  Let x = (Sync Send xc mc) in exp_sender
-  Let y = (Sync Recv xc) in exp in exp_receiver
-into 
-  Let x = (Spawn exp_receiver) in exp_sender
-
-the path to exp receiver will change from (LNext a) (LSpawn b) (LNext c) ... (LNext y) to (LSpawn x)  
-There's actually no need for subs
-
-*)
-
-(*
-
-
-inductive balanced :: "control_path \<Rightarrow> bool" where
-  Empty: "
-    balanced []
-  " |
-  Next: "
-    balanced [LNext x]
-  " |
-  CallReturn: "
-    balanced \<pi> \<Longrightarrow>
-    balanced ((LCall x) # (\<pi> ;; (LReturn x)))
-  " |
-  Append: "
-    balanced \<pi> \<Longrightarrow> balanced \<pi>' \<Longrightarrow>
-    balanced (\<pi> @ \<pi>')
-  "
-
-lemma call_return_balanced: "
-   balanced [LCall x, LReturn x]
-"
-using balanced.CallReturn balanced.Empty by fastforce
-
-
-inductive static_traceable :: "abstract_value_env \<Rightarrow> exp \<Rightarrow> control_path \<Rightarrow> exp \<Rightarrow> bool" ("_ \<turnstile> _ \<down> _ \<mapsto> _" [56,0,0,56]55)  where
-  Start: "
-    \<V> \<turnstile> e\<^sub>0 \<down> [] \<mapsto> e\<^sub>0
-  " |
-  Result: "
-    \<lbrakk>
-      \<V> \<turnstile> e\<^sub>0 \<down> \<pi> @ (LCall x) # \<pi>' \<mapsto> RESULT x\<^sub>r; 
-      balanced \<pi>';
-      \<V> \<turnstile> e\<^sub>0 \<down> \<pi> \<mapsto> LET x = b in e\<^sub>n 
-    \<rbrakk> \<Longrightarrow>
-    \<V> \<turnstile> e\<^sub>0 \<down> \<pi> @ (LCall x) # (\<pi>';;(LReturn x)) \<mapsto> e\<^sub>n
-  " |
-  Let_Unit: "
-    \<lbrakk>
-      \<V> \<turnstile> e\<^sub>0 \<down> \<pi> \<mapsto> LET x = \<lparr>\<rparr> in e\<^sub>n
-    \<rbrakk> \<Longrightarrow>
-    \<V> \<turnstile> e\<^sub>0 \<down> \<pi>;;(LNext x) \<mapsto> e\<^sub>n
-  " |
-  Let_Chan: "
-    \<lbrakk>
-      \<V> \<turnstile> e\<^sub>0 \<down> \<pi> \<mapsto> LET x = CHAN \<lparr>\<rparr> in e\<^sub>n
-    \<rbrakk> \<Longrightarrow>
-    \<V> \<turnstile> e\<^sub>0 \<down> \<pi>;;(LNext x) \<mapsto> e\<^sub>n
-  " |
-  Let_Prim: "
-    \<lbrakk>
-      \<V> \<turnstile> e\<^sub>0 \<down> \<pi> \<mapsto> LET x = Prim p in e\<^sub>n
-    \<rbrakk> \<Longrightarrow>
-    \<V> \<turnstile> e\<^sub>0 \<down> \<pi>;;(LNext x) \<mapsto> e\<^sub>n
-  " |
-  Let_Spawn_Child: "
-    \<lbrakk>
-      \<V> \<turnstile> e\<^sub>0 \<down> \<pi> \<mapsto> LET x = SPAWN e\<^sub>c in e\<^sub>n
-    \<rbrakk> \<Longrightarrow>
-    \<V> \<turnstile> e\<^sub>0 \<down> \<pi>;;(LSpawn x)  \<mapsto> e\<^sub>c
-  " |
-  Let_Spawn: "
-    \<lbrakk>
-      \<V> \<turnstile> e\<^sub>0 \<down> \<pi> \<mapsto> LET x = SPAWN e\<^sub>c in e\<^sub>n
-    \<rbrakk> \<Longrightarrow>
-    \<V> \<turnstile> e\<^sub>0 \<down> \<pi>;;(LNext x) \<mapsto> e\<^sub>n
-  " |
-  Let_Sync: "
-    \<lbrakk>
-      \<V> \<turnstile> e\<^sub>0 \<down> \<pi> \<mapsto> LET x = SYNC x\<^sub>v in e\<^sub>n
-    \<rbrakk> \<Longrightarrow>
-    \<V> \<turnstile> e\<^sub>0 \<down> \<pi>;;(LNext x) \<mapsto> e\<^sub>n
-  " |
-  Let_Fst: "
-    \<lbrakk>
-      \<V> \<turnstile> e\<^sub>0 \<down> \<pi> \<mapsto> LET x = FST p in e\<^sub>n
-    \<rbrakk> \<Longrightarrow>
-    \<V> \<turnstile> e\<^sub>0 \<down> \<pi>;;(LNext x) \<mapsto> e\<^sub>n
-  " |
-  Let_Snd: "
-    \<lbrakk>
-      \<V> \<turnstile> e\<^sub>0 \<down> \<pi> \<mapsto> LET x = SND p in e\<^sub>n
-    \<rbrakk> \<Longrightarrow>
-    \<V> \<turnstile> e\<^sub>0 \<down> \<pi>;;(LNext x) \<mapsto> e\<^sub>n
-  " |
-  Let_Case_Left: "
-    \<lbrakk>
-      \<V> \<turnstile> e\<^sub>0 \<down> \<pi> \<mapsto> LET x = CASE x\<^sub>s LEFT x\<^sub>l |> e\<^sub>l RIGHT x\<^sub>r |> e\<^sub>r in e\<^sub>n
-    \<rbrakk> \<Longrightarrow>
-    \<V> \<turnstile> e\<^sub>0 \<down> \<pi>;;(LCall x) \<mapsto> e\<^sub>l
-  " |
-  Let_Case_Right: "
-    \<lbrakk>
-      \<V> \<turnstile> e\<^sub>0 \<down> \<pi> \<mapsto> LET x = CASE x\<^sub>s LEFT x\<^sub>l |> e\<^sub>l RIGHT x\<^sub>r |> e\<^sub>r in e\<^sub>n
-    \<rbrakk> \<Longrightarrow>
-    \<V> \<turnstile> e\<^sub>0 \<down> \<pi>;;(LCall x) \<mapsto> e\<^sub>r
-  " |
-  Let_App: " 
-    \<lbrakk>
-      \<V> \<turnstile> e\<^sub>0 \<down> \<pi> \<mapsto> LET x = APP f x\<^sub>a in e\<^sub>n;
-      ^Abs f' x' e' \<in> \<V> f
-    \<rbrakk> \<Longrightarrow>
-    \<V> \<turnstile> e\<^sub>0 \<down> \<pi>;;(LCall x) \<mapsto> e'
-  "
-
-
-*)
-
 
 end
